Some initial work on proving protect/confine terminating.  However, some lemmas on Utlc well-scopedness are missing: weakening, closed terms unaffected by substitutions etc.  I also need to make OfType require that the values are closed, I think.

Compiler/ProtectConfine.v
@@ -1,22 +1,89 @@
 Require Stlc.SpecSyntax.
+Require Stlc.SpecEvaluation.
+Require Stlc.SpecTyping.
+Require Stlc.LemmasTyping.
 Require Import Utlc.SpecSyntax.
+Require Import Utlc.SpecEvaluation.
+Require Import Utlc.LemmasScoping.
+Require Import LogRel.PseudoType.
+Require Import LogRel.LR.
+Require Import Erase.
 
-Module SS := Stlc.SpecSyntax.
+Module S.
+     Include Stlc.SpecSyntax.
+     Include Stlc.SpecEvaluation.
+     Include Stlc.SpecTyping.
+     Include Stlc.LemmasTyping.
+End S.
 
-Fixpoint protect (ty : SS.Ty) : UTm :=
+Module U.
+  Include Utlc.SpecSyntax.
+  Include Utlc.SpecEvaluation.
+End U.
+
+Fixpoint protect (ty : S.Ty) : U.UTm :=
   abs (match ty with
-         | SS.tunit => var 0
-         | SS.tbool => var 0
-         | SS.tarr ty1 ty2 => abs (app (protect ty2) (app (var 1) (app (confine ty1) (var 0))))
-         | SS.tprod ty1 ty2 => pair (app (protect ty1) (proj₁ (var 0))) (app (protect ty2) (proj₂ (var 0)))
-         | SS.tsum ty1 ty2 => caseof (var 0) (inl (app (protect ty1) (var 0))) (inr (app (protect ty2) (var 0)))
+         | S.tunit => var 0
+         | S.tbool => var 0
+         | S.tarr ty1 ty2 => abs (app (protect ty2) (app (var 1) (app (confine ty1) (var 0))))
+         | S.tprod ty1 ty2 => pair (app (protect ty1) (proj₁ (var 0))) (app (protect ty2) (proj₂ (var 0)))
+         | S.tsum ty1 ty2 => caseof (var 0) (inl (app (protect ty1) (var 0))) (inr (app (protect ty2) (var 0)))
        end)
-with confine (ty : SS.Ty) : UTm :=
+with confine (ty : S.Ty) : U.UTm :=
   abs (match ty with
-         | SS.tunit => seq (var 0) unit
-         | SS.tbool => ite (var 0) true false
-         | SS.tarr ty1 ty2 => abs (app (confine ty2) (app (var 1) (app (protect ty1) (var 0))))
-         | SS.tprod ty1 ty2 => pair (app (confine ty1) (proj₁ (var 0))) (app (confine ty2) (proj₂ (var 0)))
-         | SS.tsum ty1 ty2 => caseof (var 0) (inl (app (confine ty1) (var 0))) (inr (app (confine ty2) (var 0)))
+         | S.tunit => seq (var 0) unit
+         | S.tbool => ite (var 0) true false
+         | S.tarr ty1 ty2 => abs (app (confine ty2) (app (var 1) (app (protect ty1) (var 0))))
+         | S.tprod ty1 ty2 => pair (app (confine ty1) (proj₁ (var 0))) (app (confine ty2) (proj₂ (var 0)))
+         | S.tsum ty1 ty2 => caseof (var 0) (inl (app (confine ty1) (var 0))) (inr (app (confine ty2) (var 0)))
        end).
 
+
+Local Ltac crush :=
+  repeat (try intros;
+          simpl;
+          intuition; 
+          repeat crushOfTypeUtlcMatch;
+          repeat crushUtlcScoping;
+          repeat crushUtlcSyntaxMatchH;
+          repeat crushUtlcEvaluationMatchH;
+          repeat match goal with
+                     [ |- _ ∧ _ ] => split
+                   | [ |- OfType _ _ _ ] => unfold OfType, OfTypeStlc
+                   | [ H: OfType _ _ _  |- _ ] => destruct H as [[? ?] ?]
+                   | [ H: OfTypeStlc _ _  |- _ ] => destruct H as [? ?]
+                 end;
+          S.crushTyping
+         ).
+  
+Lemma protect_confine_closed {τ} :
+  ⟨ 0 ⊢ protect τ ⟩ ∧ 
+  ⟨ 0 ⊢ confine τ ⟩.
+Proof.
+  induction τ; simpl; crush.
+  (* weakening for well-scopedness *)
+Admitted.
+  
+Lemma protect_confine_terminate {τ vu} :
+  OfTypeUtlc (embed τ) vu →
+  exists vu', U.Value vu' ∧ 
+              forall Cu, U.ECtx Cu → 
+                         (U.pctx_app (U.app (protect τ) vu) Cu) -->* (U.pctx_app vu' Cu).
+Proof.
+  revert vu.
+  induction τ; crush.
+  - (* ptarr τ₁ τ₂ *)
+    exists (abs (app (protect τ2) (app vu (app (confine τ1) (var 0))))).
+    crush. 
+    enough (U.pctx_app
+              (U.app
+                 (abs (abs (app (protect τ2) (app (var 1) (app (confine τ1) (var 0))))))
+                 vu) Cu -->
+              U.pctx_app (abs (app (protect τ2) (app vu (app (confine τ1) (var 0))))) Cu) by eauto with eval.
+    refine (U.eval_ctx₀ _ _ _); crush.
+    replace (abs (app (protect τ2) (app vu (app (confine τ1) (var 0))))) with ((abs (app (protect τ2) (app (var 1) (app (confine τ1) (var 0))))) [beta1 vu]).
+    + refine (U.eval_beta _); crush.
+    + simpl. repeat f_equal.
+      (* Problem: no assumption currently that OfType values are closed *) 
+      (* Problem: closedness implies that substitution has no effect: lemma missing? *) 
+Admitted.
